WIP

src/Reflection/Conversion.v
@@ -114,4 +114,81 @@ Section language.
       end.
     Qed.
   End mapf_id_interp.
+
+  Section mapf_interp.
+    Context {interp_base_type1 interp_base_type2 : base_type_code -> Type}
+            (interp_op1 : forall src dst, op src dst -> interp_flat_type_gen interp_base_type1 src -> interp_flat_type_gen interp_base_type1 dst)
+            (interp_op2 : forall src dst, op src dst -> interp_flat_type_gen interp_base_type2 src -> interp_flat_type_gen interp_base_type2 dst)
+            (f_var12 : forall t, interp_base_type1 t -> interp_base_type2 t)
+            (f_var21 : forall t, interp_base_type2 t -> interp_base_type1 t)
+            (f_var12_21 : forall t v, f_var12 t (f_var21 t v) = v).
+    Fixpoint f_const {t} : interp_flat_type_gen interp_base_type1 t -> interp_flat_type_gen interp_base_type2 t
+      := match t return interp_flat_type_gen interp_base_type1 t -> interp_flat_type_gen interp_base_type2 t with
+         | Tbase _ => f_var12 _
+         | Prod _ _ => fun x => (@f_const _ (fst x), @f_const _ (snd x))%core
+         end.
+    Fixpoint f_const_type {t} : interp_type interp_base_type1 t -> interp_type interp_base_type2 t
+      := match t return interp_type interp_base_type1 t -> interp_type interp_base_type2 t with
+         | Tflat _ => f_const
+         | Arrow _ _ => fun f x => @f_const_type _ (f (f_var21 _ x))
+         end.
+    Context (interp_op_Proper
+             : forall t1 tR op argsv,
+                interp_op2 t1 tR op (f_const argsv) =
+                f_const (interp_op1 t1 tR op argsv)).
+
+    Lemma interpf_mapf {t} e
+      : interpf interp_op2
+                (@mapf interp_base_type1 interp_base_type2
+                       (@f_const)
+                       _ _
+                       f_var12 f_var21
+                       t e)
+        = f_const (interpf interp_op1 e).
+    Proof.
+      induction e;
+        repeat match goal with
+               | _ => reflexivity
+               | _ => progress simpl in *
+               | _ => rewrite_hyp !*
+               | _ => apply (f_equal2 (fun x f => Let x f))
+               | _ => apply (f_equal2 (@Pair _ _))
+               | _ => apply (f_equal2 (@pair _ _))
+               | _ => solve [ eauto ]
+               end.
+      clear H IHe interp_op_Proper.
+      generalize (interpf interp_op1 e); intro x; clear e.
+      revert dependent e0; revert dependent tC; revert dependent x; induction tx; simpl;
+        [ intros; rewrite_hyp ?* | ]; intros.
+      destruct x as [x0 x1]; simpl in *.
+      lazymatch goal with
+      | [ |- f_const (interpf _ (?e0 (?x0', ?x1')%core)) = _ ]
+        => rewrite (IHtx1 x0 _ (fun x0'' => e0 (x0'', x1')%core)); cbv beta in *
+      end.
+      lazymatch goal with
+      | [ |- f_const (interpf _ (?e0 (?x0', ?x1')%core)) = _ ]
+        => apply (IHtx2 x1 _ (fun x1'' => e0 (x0', x1'')%core)); cbv beta in *
+      end.
+    Qed.
+
+    Lemma interp_map {t} e
+      : interp_type_gen_rel_pointwise
+          (interp_flat_type_gen interp_base_type2)
+          (fun _ => @eq _)
+          (interp interp_op2
+                  (@map interp_base_type1 interp_base_type2
+                        (@f_const)
+                        _ _
+                        f_var12 f_var21
+                        t e))
+          (f_const_type (interp interp_op1 e)).
+    Proof.
+      induction e;
+        repeat match goal with
+               | _ => progress simpl in *
+               | _ => progress intros
+               | _ => eauto using interpf_mapf
+               end.
+    Qed.
+  End mapf_interp.
 End language.
